Segmentation fault with to_string

cas/theories/Execute.v
@@ -1,16 +1,40 @@
+From IShrink Require Export
+     IShrink.
 From CAS Require Export
      NetUnix
-     Shrink
      Tester.
 From ExtLib Require Export
      Applicative.
 Export
   ApplicativeNotation.
 
+Variant texp : Type -> Set :=
+  Texp__Random :    texp tag
+| Texp__Var : var -> texp tag.
+
+Instance Serialize__texp : Serialize (texp tag) :=
+  fun tx => match tx with
+         | Texp__Random => Atom "Random"
+         | Texp__Var x => [Atom "Step"; to_sexp x]%sexp
+         end.
+
+Instance Serialize__reqtexp : Serialize (requestT texp) :=
+  fun m =>
+    match m with
+    | Request__GET k t =>
+      [Atom "GET"; to_sexp k; to_sexp t]
+    | Request__CAS k t v =>
+      [Atom "CAS"; to_sexp k; to_sexp t; to_sexp v]
+    end%sexp.
+
 (** Find all [n] s.t. [f (nth n l) = true]. *)
 Definition find_nth' {A} (f : A -> bool) (l : list A) : list (nat * A) :=
   let index : list nat := seq 0 $ length l in
   filter (f ∘ snd) $ zip index l.
+
+Notation stepT  := (stepT  texp requestT).
+Notation logT   := (logT   texp requestT responseT connT).
+Notation traceT := (traceT texp requestT responseT connT).
 
 Definition get_tag (sc : logT) : option tag :=
   if snd sc is Some (Response__OK t _) then Some t else None.
@@ -18,12 +42,12 @@ Definition get_tag (sc : logT) : option tag :=
 Definition has_tag (sc : logT) : bool :=
   if get_tag sc is Some _ then true else false.
 
-Definition arbitraryRequest (ss : server_state exp) (tr : traceT)
+Definition gen_step (ss : server_state exp) (tr : traceT)
   : IO stepT :=
-  let x : var := fresh_var $ script_of_trace tr in
+  let x : var := fresh_var $ map (snd ∘ fst) tr in
   k <- io_or gen_string (io_choose_ gen_string (map fst ss));;
   let ts : list (texp tag) :=
-      map (Texp__Var ∘ fst ∘ fst ∘ fst) $ filter has_tag tr in
+      map (Texp__Var ∘ fst ∘ snd ∘ fst) $ filter has_tag tr in
   t <- io_choose_ (ret Texp__Random) ts;;
   pair x <$> io_or (pure $ Request__GET k t) (Request__CAS k t <$> gen_string).
 
@@ -31,14 +55,14 @@ Definition fill_tag (tr : traceT) (tx : texp tag) : id tag :=
   match tx with
   | Texp__Random => """Random"""
   | Texp__Var x =>
-    match find (Nat.eqb x ∘ fst ∘ fst ∘ fst) tr with
-    | Some (_, _, _, Some (Response__OK _ t)) => t
+    match find (Nat.eqb x ∘ fst ∘ snd ∘ fst) tr with
+    | Some (_, _, Some (Response__OK _ t)) => t
     | _ => """Unknown"""
     end
   end.
 
-Definition fill_request (tr : traceT) (rx : requestT texp) : requestT id :=
-  match rx with
+Definition fill_request (tr : traceT) (step : stepT) : requestT id :=
+  match snd step with
   | Request__GET k tx => Request__GET k $ fill_tag tr tx
   | Request__CAS k tx v => Request__CAS k (fill_tag tr tx) v
   end.
@@ -52,27 +76,32 @@ Definition replace_first {A} (f : A -> bool) (g : A -> A) (l : list A) : list A 
   | (n, a)::_ => replace n (g a) l
   end.
 
-Definition fill_trace (c : clientT) (res : responseT id) : traceT -> traceT :=
-  replace_first (fun sc =>
-                let '(_, c0, ores) := sc in
-                if ores is None then c0 =? c else false)%nat
-             (fun sc =>
-                let '(x, req, c, _) := sc in
-                (x, req, c, Some res)).
+Definition fill_trace (p : packetT id) : traceT -> traceT :=
+  match p with
+  | Packet _ _ (inl _) => id
+  | Packet _ c (inr res) =>
+    replace_first
+      (fun sc =>
+         let '(c0, _, ores) := sc in
+         if ores is None then c0 = c? else false)%nat
+      (fun sc =>
+         let '(c, st, _) := sc in
+         (c, st, Some res))
+  end.
 
 Fixpoint findResponse (s : conn_state)
-  : IO (option (packetT id) * conn_state) :=
+  : IO (conn_state * option (packetT id)) :=
   match s with
-  | [] => ret (None, [])
+  | [] => ret ([], None)
   | (c, (f, str)) as cfs :: t =>
     match parse parseParens str with
     | inl (Some err) =>
       failwith $ "Bad response " ++ to_string str ++ " received on connection "
                ++ to_string c ++ ", error message: " ++ err
-    | inl None => '(op, t') <- findResponse t;;
-                 ret (op, cfs :: t')
+    | inl None => '(t', op) <- findResponse t;;
+                 ret (cfs :: t', op)
     | inr (r, str') =>
-      match from_string r with
+      match from_string (H:=Deserialize__responseT) r with
       | inl err =>
         failwith $ "Bad response " ++ to_string r ++ " received on connection "
                  ++ to_string c
@@ -80,85 +109,42 @@ Fixpoint findResponse (s : conn_state)
         (* prerr_endline ("================ RECEIVED =================");; *)
         let pkt := Packet Conn__Server (Conn__Client c) (inr res) in
         (* prerr_endline (to_string pkt);; *)
-        ret (Some pkt, (c, (f, str')) :: t)
+        ret ((c, (f, str')) :: t, Some pkt)
       end
     end
   end.
 
-Fixpoint execute' {R} (fuel : nat) (s : conn_state) (oscript : option scriptT)
-         (acc : traceT) (m : itree tE R)
-  : IO (bool * conn_state * traceT) :=
-  match fuel with
-  | O => ret (true, s, acc)
-  | S fuel =>
-    match observe m with
-    | RetF _ => ret (true, s, acc)
-    | TauF m' => execute' fuel s oscript acc m'
-    | VisF e k =>
-      match e with
-      | (Throw err|) => ret (false, s, acc)
-      | (|ne|) =>
-        match ne in nondetE Y return (Y -> _) -> _ with
-        | Or => fun k => b <- ORandom.bool tt;;
-                     execute' fuel s oscript acc (k b)
-        end k
-      | (||ce) =>
-        match ce in clientE Y return (Y -> _) -> _ with
-        | Client__Recv =>
-          fun k => '(op, s') <- execStateT recv_bytes s >>= findResponse;;
-                let acc' :=
-                    match op with
-                    | Some (Packet Conn__Server (Conn__Client c) (inr res)) =>
-                      fill_trace c res acc
-                    | _ => acc
-                    end in
-                execute' fuel s' oscript acc' (k op)
-        | Client__Send ss es =>
-          fun k =>
-            '(orx, ot') <- match oscript with
-                          | Some [] => ret (None, Some [])
-                          | Some (sc :: script') =>
-                            ret (Some $ sc, Some script')
-                          | None =>
-                            rx <- arbitraryRequest ss acc;;
-                            ret (Some rx, None)
-                          end;;
-            match orx with
-            | Some ((n, reqx) as step) =>
-              let req := fill_request acc reqx in
-              '(oc, s1) <- runStateT (send_request req) s;;
-              match oc with
-              | Some c =>
-                (* prerr_endline ("================== SENT ===================");; *)
-                let pkt := Packet (Conn__Client c) Conn__Server $ inl req in
-                (* prerr_endline (to_string pkt);; *)
-                execute' fuel s1 ot' (acc++[(step, c, None)])%list (k (Some pkt))
-              | None => execute' fuel s1 ot' acc (k None)
-              end
-            | None => execute' fuel s ot' acc (k None)
-            end
-        end k
-      end
-    end
-  end.
+Definition cas_tester {R} : itree tE R :=
+  tester $ observer _ $ compose_switch tcp cas_smi.
 
-Definition execute {R} (otrace : option scriptT) (m : itree tE R)
-  : IO (bool * traceT) :=
-  (* prerr_endline "<<<<< begin test >>>>>";; *)
-  '(b, s, t') <- execute' bigNumber [] otrace [] m;;
-  (* prerr_endline "<<<<<<< end test >>>>>";; *)
-  fold_left (fun m fd => OUnix.close fd;; m) (map (fst ∘ snd) s) (ret tt);;
-  ret (b, t').
+Instance Shrink__requestT : Shrink (requestT texp) := {
+  shrink _ := [] }.
 
-Definition single_test {R} (otrace : option scriptT)
-  : itree smE R -> IO (bool * traceT) :=
-  execute otrace ∘ tester ∘ observer _ ∘ compose_switch tcp.
+Arguments test : default implicits.
 
-Definition first_exec {R} : itree smE R -> IO (bool * traceT) :=
-  single_test None.
-
-Definition then_exec {R} (m : itree smE R) (init : scriptT) : IO (bool * traceT) :=
-  single_test (Some init) m.
-
-Definition test {R} (m : itree smE R) : IO bool :=
-  shrink_execute (first_exec m) (then_exec m).
+Definition test_cas : IO bool :=
+  test (expT:=texp)
+       (requestT:=requestT)
+       (responseT:=responseT)
+       Shrink__requestT
+       Serialize__reqtexp
+       Serialize__responseT
+       (connT:=connT)
+       Conn__Server
+       Serialize__connT
+       (gen_state:=server_state exp)
+       (otherE:=nondetE)
+       (fun _ e => match e with
+                | Or => ORandom.bool tt
+                end)
+       (conn_state:=conn_state)
+       []
+       fill_trace
+       fill_request
+       gen_step
+       (recv_bytes;; findResponse)
+       send_request
+       (R:=void)
+       (fun s => fold_left (fun m fd => OUnix.close fd;; m)
+                        (map (fst ∘ snd) s) (ret tt))
+       cas_tester.
