cas/theories/Common.v
@@ -3,6 +3,8 @@ From SimpleIO Require Export
      SimpleIO.
 From Parsec Require Export
      Parser.
+From QuickChick Require Export
+     Decidability.
 From ExtLib Require Export
      Functor
      Option.
@@ -21,112 +23,21 @@ Open Scope parser_scope.
 Open Scope lazy_bool_scope.
 Open Scope program_scope.
 
-Notation "P '?'" := (decide P) (at level 100).
+Instance Dec_Eq__id {A} `{Dec_Eq A} : Dec_Eq (id A).
+Proof. dec_eq. Defined.
 
-Program Instance Decidable_not {P} `{Decidable P} : Decidable (~ P) := {
-  Decidable_witness := negb (P?)
-}.
-Next Obligation.
-  intuition.
-  - apply negb_true_iff in H0.
-    eapply Decidable_complete_alt; assumption.
-  - erewrite Decidable_sound_alt; intuition.
-Qed.
-
-Notation "'Decidable_eq' A" := (forall x y : A, Decidable (x = y)) (at level 200).
-
-Program Instance Decidable_eq_id {A} `{Decidable_eq A}
-  : Decidable_eq (id A) := { Decidable_witness := @Decidable_witness (x = y) _ }.
-Next Obligation.
-  intuition; unfold Decidable_witness in *;
-    unfold Decidable_eq_id_obligation_1 in *; destruct (H x y); intuition.
-Qed.
-
-Program Instance Decidable_eq_list {A} `{Decidable_eq A}
-  : Decidable_eq (list A) := {
-  Decidable_witness :=
-    (fix eqb (x y : list A) :=
-       match x, y with
-       | [], [] => true
-       | a::x', b::y' => (a = b?) &&& eqb x' y'
-       | _, _ => false
-       end) x y }.
-Solve Obligations with split; intros; intro; intuition; discriminate.
-Next Obligation.
-  generalize dependent y.
-  induction x; destruct y; intuition; try discriminate.
-  - apply andb_true_iff in H0.
-    destruct H0.
-    f_equal.
-    + apply Decidable_spec. assumption.
-    + apply IHx. assumption.
-  - apply andb_true_iff.
-    inversion H0; subst.
-    split.
-    + apply Decidable_spec. reflexivity.
-    + apply IHx. reflexivity.
-Qed.
-
-Instance Decidable_eq_string : Decidable_eq string :=
-  { Decidable_witness := String.eqb    x y;
-    Decidable_spec    := String.eqb_eq x y }.
-
-Program Instance Decidable_eq_option {A} `{Decidable_eq A}
-  : Decidable_eq (option A) := {
-  Decidable_witness :=
-    match x, y with
-    | Some x, Some y => x = y?
-    | None  , None   => true
-    | _     , _      => false
-    end }.
-Solve Obligations with split; intuition; discriminate.
-Next Obligation.
-  destruct x, y; intuition; try discriminate;
-    f_equal; apply Decidable_spec; intuition.
-  inversion H0; reflexivity.
-Qed.
-
-Program Instance Decidable_eq_sum {A B} `{Decidable_eq A} `{Decidable_eq B}
-  : Decidable_eq (A + B) := {
-  Decidable_witness :=
-    match x, y with
-    | inl x, inl y
-    | inr x, inr y => x = y?
-    | _    , _     => false
-    end }.
-Solve Obligations with split; intuition; discriminate.
-Next Obligation.
-  intuition; try discriminate; f_equal; inversion H1;
-    apply Decidable_spec; intuition.
-Qed.
-
-Program Instance Decidable_eq_prod {A B} `{Decidable_eq A} `{Decidable_eq B}
-  : Decidable_eq (A * B) := {
-  Decidable_witness :=
-    let (xa, xb) := x in
-    let (ya, yb) := y in
-    (xa = ya?) &&& (xb = yb?) }.
-Next Obligation.
-  intuition.
-  - apply andb_true_iff in H1.
-    f_equal; apply Decidable_spec; intuition.
-  - apply andb_true_iff.
-    inversion H1.
-    intuition; apply Decidable_spec; reflexivity.
-Qed.
-
-Definition get {K V} `{Decidable_eq K} (k : K) :
+Definition get {K V} `{Dec_Eq K} (k : K) :
   list (K * V) -> option V :=
   fmap snd ∘ find ((fun kv => k = fst kv?)).
 
-Definition delete {K V} `{Decidable_eq K} (k : K) :
+Definition delete {K V} `{Dec_Eq K} (k : K) :
   list (K * V) -> list (K * V) :=
   filter (fun kv => (k <> fst kv?)).
 
 Definition put {K V} : K -> V -> list (K * V) -> list (K * V) :=
   compose cons ∘ pair.
 
-Definition update {K V} `{Decidable_eq K} (k : K) (v : V)
+Definition update {K V} `{Dec_Eq K} (k : K) (v : V)
   : list (K * V) -> list (K * V) :=
   put k v ∘ delete k.
 
