cas/theories/NetUnix.v
@@ -5,8 +5,6 @@ From SimpleIO Require Export
      IO_Float
      IO_Sys
      IO_Unix.
-From ExtLib Require Export
-     StateMonad.
 From Coq Require Export
      NArith.
 Import
@@ -37,14 +35,13 @@ Definition conn_of_fd (fd : file_descr)
 Notation BUFFER_SIZE := 1024.
 Definition SELECT_TIMEOUT := OFloat.Unsafe.of_string "0".
 
-Definition recv_bytes : stateT conn_state IO unit :=
-  mkStateT
+Definition recv_bytes : Monads.stateT conn_state IO unit :=
     (fun s =>
        '(fds, _, _) <- select (map (fst ∘ snd) s) [] [] SELECT_TIMEOUT;;
        IO.fix_io
          (fun recv_rec fds =>
             match fds with
-            | [] => ret (tt, s)
+            | [] => ret (s, tt)
             | fd :: fds' =>
               match conn_of_fd fd s with
               | Some (c, (fd, str0)) =>
@@ -52,14 +49,14 @@ Definition recv_bytes : stateT conn_state IO unit :=
                 len <- recv fd buf int_zero BUFFER_SIZE [];;
                 if len <? int_zero
                 then close fd;;
-                     ret (tt, delete c s)
+                     ret (delete c s, tt)
                 else if len =? int_zero
                      then recv_rec fds'
                      else str <- from_ostring <$> OBytes.to_string buf;;
                           let str1 : string := substring 0 (nat_of_int len) str in
                           (* prerr_endline ("Received " ++ str1 *)
                           (*                ++ " from " ++ to_string c);; *)
-                          ret (tt, update c (fd, str0 ++ str1) s)
+                          ret (update c (fd, str0 ++ str1) s, tt)
               | None => failwith "Should not happen"
               end
             end)%int (rev' fds)).
@@ -67,40 +64,34 @@ Definition recv_bytes : stateT conn_state IO unit :=
 Definition try {a b} (f : IO a) (g : IO b) : IO (option a) :=
   catch_error (Some <$> f) $ fun e m _ => g;; ret None.
 
-Definition create_conn : stateT conn_state IO (option (file_descr * clientT)) :=
-  mkStateT
-    (fun s =>
-       let iaddr : inet_addr := inet_addr_loopback in
-       port <- getport;;
-       ofd <- try (fd <- socket PF_INET SOCK_STREAM int_zero;;
-                  connect fd (ADDR_INET iaddr port);;
-                  ret fd) (ret tt);;
-       match ofd with
-       | Some fd =>
-         let c := length s in
-         ret (Some (fd, c), (c, (fd, ""))::s)
-       | None => ret (None, s)
-       end).
+Definition create_conn (s : conn_state)
+  : IO (conn_state * option (file_descr * clientT)) :=
+  let iaddr : inet_addr := inet_addr_loopback in
+  port <- getport;;
+  ofd <- try (fd <- socket PF_INET SOCK_STREAM int_zero;;
+             connect fd (ADDR_INET iaddr port);;
+             ret fd) (ret tt);;
+  match ofd with
+  | Some fd =>
+    let c := length s in
+    ret ((c, (fd, ""))::s, Some (fd, c))
+  | None => ret (s, None)
+  end.
 
-Definition send_request (req : requestT id)
-  : stateT conn_state IO (option clientT):=
-  let send_bytes fd s :=
-      let str : string := to_string req in
-      buf <- OBytes.of_string str;;
-      let len : int := OBytes.length buf in
-      IO.fix_io
-        (fun send_rec o =>
-           sent <- send fd buf o (len - o)%int [];;
-           if sent <? int_zero
-           then close fd;; ret false
-           else
-             if o + sent =? len
-             then ret true
-             else send_rec (o + sent))%int int_zero in
-  mkStateT
-    (fun s => '(ocfd, s') <- runStateT create_conn s;;
-           match ocfd with
-           | Some (fd, c) => b <- send_bytes fd s';;
-                            ret (if b : bool then Some c else None, s')
-           | None => ret (None, s')
-           end).
+Definition send_request (req : requestT id) (s : conn_state)
+  : IO (conn_state * option connT) :=
+  '(s', ofdc) <- create_conn s;;
+  if ofdc is Some (fd, c)
+  then let str : string := to_string req in
+       buf <- OBytes.of_string str;;
+       let len : int := OBytes.length buf in
+       IO.fix_io
+         (fun send_rec o =>
+            sent <- send fd buf o (len - o)%int [];;
+            if sent <? int_zero
+            then close fd;; ret (s', None)
+            else
+              if o + sent =? len
+              then ret (s', Some $ Conn__Client c)
+              else send_rec (o + sent))%int int_zero
+  else ret (s', None).
